test/KMS/Integration.dfy
@@ -36,9 +36,9 @@ module IntegTestKMS {
     var keyA :- expect UTF8.Encode("keyA");
     var valA :- expect UTF8.Encode("valA");
     var encryptionContext := map[keyA := valA];
-    assert EncryptionContext.Valid(encryptionContext) by {
-      // To prove ValidAAD, we need to reveal the definition of ValidAAD:
-      reveal EncryptionContext.Valid();
+    assert EncryptionContext.Serializable(encryptionContext) by {
+      // To prove EncryptionContext.Serializable, we need to reveal the definition of that predicate:
+      reveal EncryptionContext.Serializable();
       // We also need to help the verifier with proving the KVPairsLength is small:
       calc {
         EncryptionContext.Length(encryptionContext);
