test/SDK/Keyring/RawAESKeyring.dfy
@@ -31,7 +31,7 @@ module TestAESKeyring {
     var keyA :- expect UTF8.Encode("keyA");
     var valA :- expect UTF8.Encode("valA");
     var encryptionContext := map[keyA := valA];
-    ExpectValidAAD(encryptionContext);
+    ExpectSerializableEncryptionContext(encryptionContext);
 
     var wrappingAlgorithmID := AlgorithmSuite.AES_256_GCM_IV12_TAG16_HKDF_SHA384_ECDSA_P384;
     var signingKey := seq(32, i => 0);
@@ -56,7 +56,7 @@ module TestAESKeyring {
     var keyA :- expect UTF8.Encode("keyA");
     var valA :- expect UTF8.Encode("valA");
     var encryptionContext := map[keyA := valA];
-    ExpectValidAAD(encryptionContext);
+    ExpectSerializableEncryptionContext(encryptionContext);
 
     var pdk := seq(32, i => 0);
     var traceEntry := Materials.KeyringTraceEntry([], [], {Materials.GENERATED_DATA_KEY});
@@ -100,7 +100,7 @@ module TestAESKeyring {
     var rawAESKeyring := new RawAESKeyringDef.RawAESKeyring(name, namespace, seq(32, i => 0), EncryptionSuites.AES_GCM_256);
     var keyA :- expect UTF8.Encode("keyA");
     var unserializableEncryptionContext := generateUnserializableEncryptionContext(keyA);
-    ExpectInvalidAAD(unserializableEncryptionContext);
+    ExpectNonSerializableEncryptionContext(unserializableEncryptionContext);
 
     var wrappingAlgorithmID := AlgorithmSuite.AES_256_GCM_IV12_TAG16_HKDF_SHA384_ECDSA_P384;
     var signingKey := seq(32, i => 0);
@@ -128,7 +128,7 @@ module TestAESKeyring {
 
     // Set up EC that can't be serialized
     var unserializableEncryptionContext := generateUnserializableEncryptionContext(keyA);
-    ExpectInvalidAAD(unserializableEncryptionContext);
+    ExpectNonSerializableEncryptionContext(unserializableEncryptionContext);
     var verificationKey := seq(32, i => 0);
 
     var decryptionMaterialsIn := Materials.DecryptionMaterials.WithoutPlaintextDataKey(unserializableEncryptionContext, wrappingAlgorithmID, Some(verificationKey));
